Reworked to do imperative state updates instead of message passing.

notes/Concurrent.v
@@ -1,115 +1,132 @@
 Require Import Arith Bool List String CpdtTactics.
-
-Definition tid := nat.
-Definition msg := string.
-
-Inductive com : Type -> Type := 
-| Ret : forall {A}, A -> com A
-| Bind : forall {A B}, com A -> (A -> com B) -> com B
-| Send : tid -> msg -> com unit
-| Rcv : com string.
-
-Inductive system := 
-| Empty : system
-| Thread : tid -> com unit -> system
-| Par : system -> system -> system.
-
-Infix "|+|" := Par (right associativity, at level 80).
-
-Reserved Notation "s1 ~~ s2" (at level 84).
-
-Inductive equiv : system -> system -> Prop := 
-| system_refl : forall s, s ~~ s
-| system_trans : forall s1 s2 s3, s1 ~~ s2 -> s2 ~~ s3 -> s1 ~~ s3
-| system_comm : forall s1 s2, s1 |+| s2 ~~ s2 |+| s1
-| system_assoc : forall s1 s2 s3,
-                   s1 |+| (s2 |+| s3) ~~ (s1 |+| s2) |+| s3
-| system_plus_empty : forall s, equiv (s |+| Empty) s
-| system_cong : forall s1 s2 s3 s4, 
-                  s1 ~~ s3 -> s2 ~~ s4 -> s1 |+| s2 ~~ s3 |+| s4
-where "s1 ~~ s2" := (equiv s1 s2).
-
-Inductive action : Type := 
-| Eps_a : action
-| Send_a : tid -> msg -> action
-| Rcv_a : msg -> action
-| Fork_a : tid -> com unit -> action.
-
-Reserved Notation "c1 -: a :-> c2" (at level 84).
-
-Inductive step_thread : forall {A}, com A -> action -> com A -> Prop := 
-| step_Ret_Bind : 
-    forall {A B} (x:A) (f:A -> com B), 
-      (Bind (Ret x) f) -:Eps_a:-> (f x)
-| step_Cong : 
-    forall {A B} (c:com A) (a: action) (c':com A) (f: A -> com B),
-      c -:a:-> c' -> Bind c f -:a:-> Bind c' f
-| step_Send : 
-    forall (t:tid) (m:msg), 
-      Send t m -:Send_a t m:-> Ret tt
-| step_Rcv : 
-    forall (m:msg), 
-      Rcv -:Rcv_a m:-> Ret m
-where "c1 -: a :-> c2" := (step_thread c1 a c2).
-
-Reserved Notation "s1 ==> s2" (at level 84).
-
-Inductive step_system : system -> system -> Prop := 
-| system_Eps : 
-    forall t c1 c1', 
-      c1 -:Eps_a:-> c1' -> 
-      Thread t c1 ==> Thread t c1'
-| system_SndRcv : 
-    forall t1 c1 c1' 
-           t2 c2 c2' m,
-      c1 -: (Send_a t2 m) :-> c1' -> 
-      c2 -: (Rcv_a m) :-> c2' -> 
-      Thread t1 c1 |+| Thread t2 c2 ==>
-      Thread t1 c1' |+| Thread t2 c2'
-| system_GC : 
-    forall t, 
-      Thread t (Ret tt) ==> Empty
-| system_Cong : 
-    forall s1 s1' s2,
-      s1 ==> s1' -> s1 |+| s2 ==> s1' |+| s2
-| system_Equiv : 
-    forall s1 s2 s3 s4,
-      s1 ==> s2 -> s1 ~~ s3 -> s2 ~~ s4 -> s3 ==> s4
-where "s1 ==> s2" := (step_system s1 s2).
-
+Local Open Scope string_scope.
+Infix "++" := List.app.
+Import ListNotations.
 Class Monad(M:Type -> Type) := 
 {
   ret : forall {A:Type}, A -> M A ; 
   bind : forall {A B:Type}, M A -> (A -> M B) -> M B
 }.
+Notation "x <- c1 ; c2" := (bind c1 (fun x => c2))
+  (right associativity, at level 84, c1 at next level).
 
-Definition ready_queue := list (tid * (com unit))%type.
-
-Definition M (A:Type) := tid -> (A -> com unit) -> ready_queue -> list (ready_queue).
-
-Definition MReturn {A:Type} (x:A) : M A := 
-  fun (t:tid) (k: A -> com unit) (q:ready_queue) => 
-    ((t, k x)::q)::nil.
-
-Definition MBind {A B:Type} (c:M A) (f:A -> M B) : M B := 
-  fun (t:tid) (k: B -> com unit) (q:ready_queue) => 
-    c t (fun (v:A) => Bind (Ret v) c)
-  
 Definition flatMap {A B:Type} (xs:list A) (f:A->list B) : list B := 
   fold_right (fun x a => (f x) ++ a) nil xs.
 
-Instance mMonad : Monad M := 
-{
-  ret := fun {A:Type} (x:A) (t:tid) (k:A-> com unit)(r:ready_queue) => (x::nil) ; 
-  bind := @flatMap
-}.
+Definition var := string.
+Definition lock := string.
+Definition value := nat.
+Definition store := list (var * value).
+Inductive lock_state := Locked | Unlocked.
+Definition locks := list (var * lock_state).
+Definition memory := (locks * store)%type.
 
-Fixpoint step_thread_fn {A} (c:com A) : list (com A) := 
-  match c with 
-    | Ret v => 
-    | Bind c f => 
-  
+Fixpoint update {A} (v:string) (val:A) (m:list (string * A)) : list (string * A) := 
+  match m with 
+    | nil => (v,val)::nil
+    | (v',val')::m' => if string_dec v v' then (v',val)::m'
+                       else (v',val')::(update v val m')
+  end.
 
-(* As usual, we will use the more convenient notation for bind. *)
-Notation "x <- c1 ; c2" := (bind c1 (fun x => c2)) 
+Fixpoint lookup_def {A} (v:var) (m:list (string * A)) (def:A) : A := 
+  match m with 
+    | nil => def
+    | (v',val)::m' => if string_dec v v' then val else lookup_def v m' def
+  end.
+
+Definition lookup_lock (l:lock) (m:memory) : lock_state := 
+  lookup_def l (fst m) Unlocked.
+
+Definition lookup_store (v:var) (m:memory) : value := 
+  lookup_def v (snd m) 0.
+
+Definition update_store (v:var) (val:value) (m:memory) : memory := 
+  (fst m, update v val (snd m)).
+
+Definition update_lock (l:lock) (ls:lock_state) (m:memory) : memory := 
+  (update l ls (fst m), snd m).
+
+Inductive com : Type := 
+| Ret : value -> com
+| Bind : com -> (value -> com) -> com
+| Write : var -> value -> com
+| Read : var -> com
+| Lock : lock -> com
+| Unlock : lock -> com.
+
+Definition program := list com.
+
+Notation "'def' x ':=' c1 'in' c2" := (Bind c1 (fun x => c2))
   (right associativity, at level 84, c1 at next level).
+Definition c1 : com := def v := Read "x" in Write "x" (1 + v).
+Definition c2 : com := def v := Read "x" in Write "x" (v - 1).
+Definition c3 : com := def v := Read "x" in if eq_nat_dec v 0 then Write "y" 42 else  Write "y" 1.
+
+Definition p0 : program := [c1;c2;c3].
+Definition s0 : store := [("x",0) ; ("y",0)].
+Definition l0 : locks := [].
+Definition m0 : memory := (l0, s0).
+
+Inductive step_com : com -> memory -> com -> memory -> Prop := 
+| step_bind_ret : forall v f m, step_com (Bind (Ret v) f) m (f v) m
+| step_bind_cong : forall c c' m m' f, 
+                     step_com c m c' m' -> 
+                     step_com (Bind c f) m (Bind c' f) m'
+| step_write : forall x v m m', m' = update_store x v m -> step_com (Write "x" v) m (Ret v) m'
+| step_read : forall x m v, v = lookup_store x m -> step_com (Read "x") m (Ret v) m
+| step_lock : forall l m m', lookup_lock l m = Unlocked -> m' = update_lock l Locked m -> 
+                             step_com (Lock l) m (Ret 1) m'
+| step_unlock : forall l m m', lookup_lock l m = Locked -> m' = update_lock l Unlocked m -> 
+                               step_com (Unlock l) m (Ret 1)  m'.
+Hint Constructors step_com.
+
+Inductive step_program : program -> memory -> program -> memory -> Prop := 
+| step_prog_com : forall cs1 c cs2 m c' m' p1 p2,
+                    step_com c m c' m' -> 
+                    p1 = cs1 ++ c :: cs2 -> 
+                    p2 = cs1 ++ c' :: cs2 -> 
+                    step_program p1 m p2 m'
+| step_prog_gc : forall cs1 cs2 v m, 
+                   step_program (cs1 ++ (Ret v) :: cs2) m (cs1 ++ cs2) m.
+Hint Constructors step_program.
+
+Inductive rt_step_program : program -> memory -> program -> memory -> Prop := 
+| rt_step : forall p1 m1 p2 m2 p3 m3, 
+              step_program p1 m1 p2 m2 -> 
+              rt_step_program p2 m2 p3 m3 -> 
+              rt_step_program p1 m1 p3 m3
+| rt_refl : forall p m, rt_step_program p m p m.
+Hint Constructors rt_step_program.
+
+Definition evals : program -> memory -> memory -> Prop := 
+  fun p1 m1 m2 => rt_step_program p1 m1 nil m2.
+
+Fixpoint step_com_fn' (c:com) (m:memory) : option (com * memory) := 
+  match c with 
+    | Ret _ => None
+    | Bind (Ret v) f => Some (f v, m)
+    | Bind c1 f => match step_com_fn' c1 m with
+                     | None => None
+                     | Some (c2, m') => Some (Bind c2 f, m')
+                   end
+    | Write x v => Some (Ret v, update_store x v m)
+    | Read x => Some (Ret (lookup_store x m), m)
+    | Lock l => match lookup_lock l m with 
+                  | Unlocked => Some (Ret 1, update_lock l Locked m)
+                  | Locked => None
+                end
+    | Unlock l => match lookup_lock l m with 
+                  | Locked => Some (Ret 1, update_lock l Unlocked m)
+                  | Unlocked => None
+                  end
+  end.
+
+
+Lemma p0_trace1 : evals p0 m0 (nil,[("x",0) ; ("y",42)]).
+Proof.
+  Admitted.
+
+
+
+
+
